Clean up things

Autoinc/SequenceTree.lean
@@ -1,40 +1,40 @@
 import Plausible
 import Autoinc.Sequence
 
-section Tree
+section SequenceTree
 
 -- sequence represented as a 2-3 tree
-inductive Tree (α : Type) where
+inductive SequenceTree (α : Type) where
   | Empty
   | Leaf (val : α)
-  | Node2 (height : Nat) (size : Nat) (left right : Tree α)
-  | Node3 (height : Nat) (size : Nat) (left middle right : Tree α)
+  | Node2 (height : Nat) (size : Nat) (left right : SequenceTree α)
+  | Node3 (height : Nat) (size : Nat) (left middle right : SequenceTree α)
 deriving BEq
 
-def Tree.height : Tree α → Nat
+def SequenceTree.height : SequenceTree α → Nat
   | Empty | Leaf _ => 0
   | Node2 h _ _ _ | Node3 h _ _ _ _ => h
 
-def Tree.size : Tree α → Nat
+def SequenceTree.size : SequenceTree α → Nat
   | Empty => 0
   | Leaf _ => 1
   | Node2 _ size _ _ | Node3 _ size _ _ _ => size
 
 -- assumption: l.height == r.height
-def mkNode2 (l r : Tree α) : Tree α :=
+def mkNode2 (l r : SequenceTree α) : SequenceTree α :=
   .Node2 (l.height + 1) (l.size + r.size) l r
 
 -- assumption: l.height == m.height == r.height
-def mkNode3 (l m r : Tree α) : Tree α :=
+def mkNode3 (l m r : SequenceTree α) : SequenceTree α :=
   .Node3 (l.height + 1) (l.size + m.size + r.size) l m r
 
-def combine : List (Tree α) → List (Tree α)
+def combine : List (SequenceTree α) → List (SequenceTree α)
   | [a, b] => [mkNode2 a b]
   | [a, b, c] => [mkNode3 a b c]
   | [a, b, c, d] => [mkNode2 a b, mkNode2 c d]
   | _ => panic! "invalid level up state"
 
-def mergeToSameHeight (a b : Tree α) : List (Tree α) :=
+def mergeToSameHeight (a b : SequenceTree α) : List (SequenceTree α) :=
   let heightA := a.height
   let heightB := b.height
   if heightA < heightB then
@@ -52,7 +52,7 @@ def mergeToSameHeight (a b : Tree α) : List (Tree α) :=
   else
     [a, b]
 
-def Tree.merge : Tree α → Tree α → Tree α
+def SequenceTree.merge : SequenceTree α → SequenceTree α → SequenceTree α
   | a, Empty => a
   | Empty, b => b
   | a, b => match mergeToSameHeight a b with
@@ -60,8 +60,7 @@ def Tree.merge : Tree α → Tree α → Tree α
     | [t, u] => mkNode2 t u
     | _ => .Empty -- invalid state, TODO: find cleaner solution
 
-/-- splits the tree at an index -/
-def Tree.split (i : Nat) : Tree α → (Tree α) × (Tree α)
+def SequenceTree.split (i : Nat) : SequenceTree α → (SequenceTree α) × (SequenceTree α)
   | Empty => (Empty, Empty)
   | Leaf x => if i == 0 then (Empty, Leaf x) else (Leaf x, Empty)
   | Node2 _ _ l r =>
@@ -92,19 +91,19 @@ def Tree.split (i : Nat) : Tree α → (Tree α) × (Tree α)
         let (r1, r2) := r.split (i' - sizeM)
         (l.merge (mkNode2 m r1), r2)
 
-def Tree.insert (t : Tree α) (i : Nat) (x : α) : Tree α :=
+def SequenceTree.insert (t : SequenceTree α) (i : Nat) (x : α) : SequenceTree α :=
   let (l, r) := t.split i
   l.merge (Leaf x) |>.merge r
 
-def Tree.delete (t : Tree α) (i : Nat) : Tree α :=
+def SequenceTree.delete (t : SequenceTree α) (i : Nat) : SequenceTree α :=
   let (l, r) := t.split i
   let (_, r2) := r.split 1
   l.merge r2
 
-def Tree.push (t : Tree α) (x : α) : Tree α :=
+def SequenceTree.push (t : SequenceTree α) (x : α) : SequenceTree α :=
   t.insert t.size x
 
-def fromListAux (remaining : List (Tree α)) (acc: List (Tree α)) (flip : Bool) : Tree α :=
+def fromListAux (remaining : List (SequenceTree α)) (acc: List (SequenceTree α)) (flip : Bool) : SequenceTree α :=
   match remaining, acc with
   | [], _ => .Empty
   | [a], _ => a
@@ -130,30 +129,30 @@ def fromListAux (remaining : List (Tree α)) (acc: List (Tree α)) (flip : Bool)
     fromListAux remaining (node :: acc) flip
 termination_by remaining.length + acc.length
 
-def Tree.fromList (xs : List α) : Tree α :=
+def SequenceTree.fromList (xs : List α) : SequenceTree α :=
   fromListAux (xs.map (.Leaf ·)) [] false
 
-def Tree.fromList' (xs : List α) : Tree α :=
+def SequenceTree.fromList' (xs : List α) : SequenceTree α :=
   xs.foldl (fun t x => t.push x) .Empty -- this is horribly slow
 
-def Tree.toList (t : Tree α) : List α :=
+def SequenceTree.toList (t : SequenceTree α) : List α :=
   prepend t []
     where
-  prepend : Tree α → List α → List α
+  prepend : SequenceTree α → List α → List α
   | Empty, xs => xs
   | Leaf x, xs => x :: xs
   | Node2 _ _ l r, xs => prepend l (prepend r xs)
   | Node3 _ _ l m r, xs => prepend l (prepend m (prepend r xs))
 
 -- TODO: is fold the correct term here?
-def Tree.foldl (t : Tree α) (f : β → α → β) (init : β) :=
+def SequenceTree.foldl (t : SequenceTree α) (f : β → α → β) (init : β) :=
   match t with
   | Empty => init
   | Leaf x => f init x
   | Node2 _ _ l r => foldl l f (foldl r f init)
   | Node3 _ _ l m r => foldl l f (foldl m f (foldl r f init))
 
-partial def foldlTRAux (f : β → α → β) (init : β) (remaining : List (Tree α)) : β :=
+partial def foldlTRAux (f : β → α → β) (init : β) (remaining : List (SequenceTree α)) : β :=
   match remaining with
   | [] => init
   | .Empty :: remaining => foldlTRAux f init remaining
@@ -161,27 +160,27 @@ partial def foldlTRAux (f : β → α → β) (init : β) (remaining : List (Tre
   | .Node2 _ _ l r :: remaining => foldlTRAux f init (l :: r :: remaining)
   | .Node3 _ _ l m r :: remaining => foldlTRAux f init (l :: m :: r :: remaining)
 
-def Tree.foldlTR (t : Tree α) (f : β → α → β) (init : β) :=
+def SequenceTree.foldlTR (t : SequenceTree α) (f : β → α → β) (init : β) :=
   foldlTRAux f init [t]
 
-def Tree.count [BEq α] (t : Tree α) (x : α) : Nat :=
+def SequenceTree.count [BEq α] (t : SequenceTree α) (x : α) : Nat :=
   t.foldlTR (fun acc y => if x == y then acc + 1 else acc) 0
 
-def Tree.getRange (t : Tree α) (i n : Nat) : Tree α :=
+def SequenceTree.getRange (t : SequenceTree α) (i n : Nat) : SequenceTree α :=
   let (_, r) := t.split i
   r.split n |>.1
 
-def Tree.insertList (t : Tree α) (i : Nat) (xs : List α) : Tree α :=
-  let txs := Tree.fromList xs
+def SequenceTree.insertList (t : SequenceTree α) (i : Nat) (xs : List α) : SequenceTree α :=
+  let txs := SequenceTree.fromList xs
   let (l, r) := t.split i
   l.merge txs |>.merge r
 
-def Tree.deleteRange (t : Tree α) (i n : Nat) : Tree α :=
+def SequenceTree.deleteRange (t : SequenceTree α) (i n : Nat) : SequenceTree α :=
   let (l, r) := t.split i
   let (_, rr) := r.split n
   l.merge rr
 
-def Tree.fold (t : Tree α) (fempty : β) (fleaf : α → β) (fnode2 : β → β → β) (fnode3 : β → β → β → β) :=
+def SequenceTree.fold (t : SequenceTree α) (fempty : β) (fleaf : α → β) (fnode2 : β → β → β) (fnode3 : β → β → β → β) :=
   match t with
   | Empty => fempty
   | Leaf x => fleaf x
@@ -195,30 +194,42 @@ def Tree.fold (t : Tree α) (fempty : β) (fleaf : α → β) (fnode2 : β → �
       (m.fold fempty fleaf fnode2 fnode3)
       (r.fold fempty fleaf fnode2 fnode3)
 
-def Tree.patchWith (t : Tree α) (f : α → β → α) (ds : List β) : Tree α :=
-  -- TODO: look for more optimal ways (its gonna be O(n) either way but maybe we can reduce it by a constant factor of 2-3)
-  Tree.fromList <| t.toList |>.zipWith f ds
+def SequenceTree.patchWith (t : SequenceTree α) (f : α → β → α) (ds : List β) : SequenceTree α :=
+  let rec helper : SequenceTree α → List β → ((SequenceTree α) × List β)
+    | t, [] => (t, [])
+    | Empty, ds => (Empty, ds)
+    | Leaf x, d :: ds => (Leaf (f x d), ds)
+    | Node2 h s l r, ds =>
+      let (patchedL, ds') := helper l ds
+      let (patchedR, ds'') := helper r ds'
+      (Node2 h s patchedL patchedR, ds'')
+    | Node3 h s l m r, ds =>
+      let (patchedL, ds') := helper l ds
+      let (patchedM, ds'') := helper m ds'
+      let (patchedR, ds''') := helper r ds''
+      (Node3 h s patchedL patchedM patchedR, ds''')
+  helper t ds |>.1
 
-instance : Sequence α (Tree α) where
-  fromList := Tree.fromList
-  toList := Tree.toList
-  insert := Tree.insert
-  delete := Tree.delete
+instance : Sequence α (SequenceTree α) where
+  fromList := SequenceTree.fromList
+  toList := SequenceTree.toList
+  insert := SequenceTree.insert
+  delete := SequenceTree.delete
   splitAt t i := t.split i
-  length := Tree.size
-  count := Tree.count
-  getRange := Tree.getRange
-  insertList := Tree.insertList
-  deleteRange := Tree.deleteRange
-  concat := Tree.merge
-  patchWith := Tree.patchWith
+  length := SequenceTree.size
+  count := SequenceTree.count
+  getRange := SequenceTree.getRange
+  insertList := SequenceTree.insertList
+  deleteRange := SequenceTree.deleteRange
+  concat := SequenceTree.merge
+  patchWith := SequenceTree.patchWith
 
-instance : Inhabited (Tree α) where
+instance : Inhabited (SequenceTree α) where
   default := .Empty
 
-end Tree
+end SequenceTree
 
-namespace Tree.Tests
+namespace SequenceTree.Tests
 
 open Plausible in
 instance : Arbitrary (Fin n) where
@@ -237,38 +248,38 @@ abbrev α := Nat
 
 -- toList is inverse to fromList
 example (xs : List α) :
-  (Tree.fromList xs |>.toList) == xs
+  (SequenceTree.fromList xs |>.toList) == xs
 := by plausible
 
 -- tree has correct size
 example (xs : List α) :
-  (Tree.fromList xs |>.size) == xs.length
+  (SequenceTree.fromList xs |>.size) == xs.length
 := by plausible
 
 -- push works
 example (xs : List α) (x : α) :
-  let t := Tree.fromList xs |>.push x
+  let t := SequenceTree.fromList xs |>.push x
   let xs' := xs ++ [x]
   t.toList == xs'
 := by plausible
 
 -- insert works
 example (xs : List α) (i : Fin (xs.length)) (x : α) :
-  let t := Tree.fromList xs |>.insert i x
+  let t := SequenceTree.fromList xs |>.insert i x
   let xs' := xs.insertIdx i x
   t.toList == xs'
 := by plausible
 
 -- delete works
 example (xs : List α) (i : Fin (xs.length)) :
-  let t := Tree.fromList xs |>.delete i
+  let t := SequenceTree.fromList xs |>.delete i
   let (xs₁, xs₂) := xs.splitAt i
   t.toList == xs₁ ++ xs₂.tail
 := by plausible
 
 -- foldlTR = foldl
 example (xs : List α) :
-  let t := Tree.fromList xs
+  let t := SequenceTree.fromList xs
   let f := (fun acc y => if x == y then acc + 1 else acc)
   let resTR := t.foldlTR f 0
   let resNTR := t.foldl f 0
@@ -277,7 +288,7 @@ example (xs : List α) :
 
 -- fromList = fromList'
 example (xs : List α) :
-  (Tree.fromList xs |>.toList) == (Tree.fromList' xs |>.toList)
+  (SequenceTree.fromList xs |>.toList) == (SequenceTree.fromList' xs |>.toList)
 := by plausible
 
-end Tree.Tests
+end SequenceTree.Tests
