Benchmark/Sequence.lean
@@ -11,7 +11,6 @@ def forceSequence [Sequence β γ] (s : γ) : IO Nat := do
   let t₂ ← IO.monoNanosNow
   return t₂ - t₁
 
--- benchmark patching list with changes vs patching tree with changes
 def benchmark [Sequence β γ] (f : α → γ) (input : α) (rep : Nat := 50) : IO Float := do
   let mut total : UInt64 := 0
   for _ in [0:rep] do
@@ -33,23 +32,12 @@ def inputSize := 10000
 def input := List.range inputSize
 def changeSize := 5.0 -- %
 
-def exec [Sequence β γ] (name : String) (f : ΔList Nat ΔNat → γ) (inputs : List (String × ΔList Nat ΔNat)) : IO Unit := do
-  let unnamedInputs := inputs.map (·.2)
-  let inputNames := inputs.map (·.1)
-  IO.println name
-  IO.println "------"
-  let results ← benchmarkList f unnamedInputs
-  let namedResults := inputNames.zip results
-  for (inputName, t) in namedResults do
-    IO.println s!"{inputName} | {t.trunc 3}ns"
-  IO.println "------"
-
 def at_p (p : Float) (size : Nat) : Nat :=
   p * size.toFloat |>.toUInt64 |>.toNat
 
-def execAll : IO Unit := do
+def execAll (caption : Option String := none) : IO Unit := do
   let list := Sequence.fromList (γ := List Nat) input
-  let tree := Sequence.fromList (γ := Tree Nat) input
+  let tree := Sequence.fromList (γ := SequenceTree Nat) input
   let size := (changeSize / 100.0) * inputSize.toFloat |> (·.toUInt64.toNat)
   let gen ← IO.stdGenRef.get
   let inputs := [
@@ -66,9 +54,6 @@ def execAll : IO Unit := do
     ("Update at the end of the list", randUpd (at_p 0.8 inputSize) (at_p 0.9 inputSize) size gen |>.1),
   ]
 
-  exec "List" (list ⨁ ·) inputs
-  exec "Tree" (tree ⨁ ·) inputs
-
   let inputNames := inputs.map (·.1)
   let inputValues := inputs.map (·.2)
   let listTimes ← benchmarkList (list ⨁ ·) inputValues
@@ -83,4 +68,4 @@ def execAll : IO Unit := do
     |>.zip (speedups.map (·.trunc))
     |>.map (fun (((n, l), t), s) => [n, l, t, s])
 
-  printTable headers rows
+  printTable headers rows (caption := caption)
